During the first of the 2 atomic moves in Wriggle, the car's leftmost point shifts right. (Hence it suffices to consider to consider the intial position for this move, for computing space requirements)

src/robots/car/ackermannSteeringProp.v
@@ -121,8 +121,6 @@ Qed.
 (**width needs to be nonzero so that we can take its reciprocal in an arctan.
   others can also be required to be strictly positive*)
 
-Definition nonTrivialCarDim (cd : CarDimensions IR) :=
-  0 ≤ lengthFront cd  and  0 [<] width cd and 0 ≤ lengthBack cd.
 
 Global Instance EquivalenceCarDim  `{e:Equiv A}
   `{Equivalence _ e}
